theories/case_studies/mt/domain_manager.v
@@ -1,4 +1,3 @@
-
 From iris.proofmode Require Import base tactics classes.
 From iris.algebra Require Import excl excl_auth gset gmap agree csum frac excl.
 From iris.base_logic Require Import invariants.
@@ -8,43 +7,246 @@ From program_logic Require Import reasoning_rules.
 From case_studies.eio Require Import eio.
 From case_studies.mt Require Import spawn.
 
-
-(* Proof-of-concept spawn function that blocks the thread. *)
-Definition spawn_scheduler : val := 
+Definition make_register : val :=
+  (λ: "domain" "init" "f", (λ: "waker",
+      let: "new_scheduler" := (λ: <>, 
+        let: "result" := run "init" "f" in
+        "waker" #();;
+        "result"
+      ) in
+      let: "joinh" := spawn "new_scheduler" in
+      "domain" <- SOME "joinh"
+  ))%V.
+Definition spawn_scheduler2 : val :=
   (λ: "init" "f",
-    let: "new_scheduler" := (λ: <>, run "init" "f") in
-    let: "c" := spawn "new_scheduler" in
-    join "c")%V.
+    let: "domain" := ref NONEV in
+    let: "register" := make_register "domain" "init" "f" in
+    suspend "register";;
+    match: Load "domain" with
+      NONE => #() #()
+    | SOME "joinh" => join "joinh"
+    end)%V.
+
+Class domainG Σ := DomainG { 
+  domain_tokG : inG Σ (exclR unitO)
+}.
+Local Existing Instance domain_tokG.
+
+Definition domainΣ : gFunctors := #[GFunctor (exclR unitO)].
+
+Global Instance subG_domainΣ {Σ} : subG domainΣ Σ → domainG Σ.
+Proof. solve_inG. Qed.
+
+Section spec.
+  Context `{!heapGS Σ, !spawnG Σ, !promiseGS Σ, !domainG Σ}.
+  Context (N Njoin: namespace).
+
+  Definition domain_state_fresh γ := own γ (Cinl 1%Qp).
+  Definition domain_state_unset γ := own γ (Cinl (1/2)%Qp).
+  Definition domain_state_set γ := own γ (Cinr (to_agree #())).
+
+  Definition domain_inv γ δ ℓ Φ := (
+    ∃ v, ℓ ↦ v ∗ (
+      (⌜ v = NONEV ⌝ ∗ domain_state_unset γ)
+    ∨ (∃ (ℓ' : loc), ⌜ v = SOMEV #ℓ' ⌝ ∗ domain_state_set γ ∗ (join_handle Njoin ℓ' (λ v, □ Φ v)%I ∨ own δ (Excl ())))
+  ))%I.
+
+  Definition is_domain_ref γ δ ℓ Φ := inv N (domain_inv γ δ ℓ Φ).
+  Definition domain_handle γ δ ℓ Φ := (
+    own δ (Excl ()) ∗ is_domain_ref γ δ ℓ Φ
+  )%I.
+
+  Global Instance domain_state_set_Persistent γ : Persistent (domain_state_set γ).
+  Proof. by apply _. Qed.
+
+  Lemma domain_state_fresh_create : ⊢ |==> ∃ γ, domain_state_fresh γ.
+  Proof. by iMod (own_alloc (Cinl 1%Qp)) as (γ) "Hps"; last iExists γ. Qed.
+
+  Lemma domain_state_split γ :
+    ⊢ domain_state_fresh γ ==∗ domain_state_unset γ ∗ domain_state_unset γ.
+  Proof.
+    rewrite /domain_state_fresh /domain_state_unset.
+    rewrite -own_op.
+    iApply own_update.
+    rewrite -Cinl_op.
+    apply csum_update_l.
+    rewrite frac_op.
+    rewrite cmra_update_updateP.
+    apply cmra_updateP_id. 
+    apply Qp_half_half.
+  Qed. 
+
+  Lemma domain_state_join γ :
+    ⊢ domain_state_unset γ ∗ domain_state_unset γ ==∗ domain_state_fresh γ.
+  Proof.
+    rewrite /domain_state_fresh /domain_state_unset.
+    rewrite -own_op.
+    iApply own_update.
+    rewrite -Cinl_op.
+    apply csum_update_l.
+    rewrite frac_op.
+    rewrite cmra_update_updateP.
+    apply cmra_updateP_id. 
+    by rewrite Qp_half_half.
+  Qed.
+
+  Lemma domain_state_create ℓ Φ :
+    ⊢ ℓ ↦ NONEV ={⊤}=∗ ∃ γ δ, domain_handle γ δ ℓ Φ ∗ domain_state_unset γ.
+  Proof.
+    iIntros "Hℓ".
+    iMod (domain_state_fresh_create) as "(%γ & Hds)".
+    iMod (domain_state_split with "Hds") as "(Hds & Hds')".
+    iMod (own_alloc (Excl ())) as (δ) "Hδ"; first done.
+    iExists γ, δ.
+    iFrame. 
+    iApply (inv_alloc _ _ (domain_inv γ δ ℓ Φ) with "[Hℓ Hds]").
+    iNext. rewrite /domain_inv.
+    iExists NONEV. iFrame.
+    iLeft. by iFrame.
+  Qed.
+
+  Lemma domain_state_fulfill γ :
+    ⊢ domain_state_fresh γ ==∗ domain_state_set γ.
+  Proof.
+    iApply own_update.
+    apply cmra_update_exclusive.
+    apply Cinr_valid.
+    done.
+  Qed.
+  
+  Lemma domain_state_disjoint γ : 
+    ⊢ domain_state_unset γ -∗ domain_state_set γ -∗ False.
+  Proof. 
+    iIntros "H1 H2".
+    rewrite /domain_state_unset /domain_state_set.
+    iPoseProof (own_valid_2 with "H1 H2") as "H".
+    by rewrite csum_validI.
+  Qed.
+End spec.
       
 Section proof.
-Context `{!heapGS Σ, !spawnG Σ, !promiseGS Σ, !savedPredG Σ val}.
-Context (N : namespace).
-(* What would the specification of spawn_scheduler be? 
-  Nothing interesting I think since it just wraps run.
+  Context `{!heapGS Σ, !spawnG Σ, !promiseGS Σ, !savedPredG Σ val, !domainG Σ}.
+  Context (N Njoin : namespace).
 
-  EWP f #() <| Ψ |> {{ Q }}
-  ---------------------
-  EWP (spawn_scheduler f) <| ⊥ |> {{ Q }}
-*)
+  Lemma make_register_spec γ δ ℓ (I Φ : val -> iProp Σ) (init f: val) :
+    ⊢ promiseInv -∗ 
+      I init -∗ 
+      (∀ δℓ, isTlvPred δℓ.1.1.2 I -∗ fiberResources (fst δℓ) (snd δℓ) -∗ EWP (f #()) <| Coop δℓ |> {{ v, □ Φ v ∗ fiberResources (fst δℓ) (snd δℓ) }}) -∗
+      is_domain_ref N Njoin γ δ ℓ Φ -∗ 
+      domain_state_unset γ -∗
+        EWP (make_register #ℓ init f) <| ⊥ |> {{reg, 
+          ∀ (waker: val), (∀ (v: val), □ True -∗ EWP (waker v) <| ⊥ |> {{_, True }}) -∗
+            (▷ EWP (reg waker) <| ⊥ |> {{_, □ domain_state_set γ }}) }}.
+  Proof.
+    iIntros "HInv Hinit Hf Hdr Hγ". rewrite /make_register.
+    ewp_pure_steps.
+    iIntros (waker) "Hwaker !>".
+    ewp_pure_steps.
+    (* spawn the new thread *)
+    ewp_bind_rule; simpl.
+    iApply (ewp_mono with "[Hwaker HInv Hinit Hf]").
+    { iApply (spawn_spec Njoin (λ v, □ Φ v)%I with "[Hwaker HInv Hinit Hf]").
+      ewp_pure_steps.
+      iApply (ewp_bind' (AppRCtx _)); [by done|simpl].
+      iApply (ewp_mono with "[HInv Hinit Hf]").
+      { iApply (ewp_run _ _ I Φ). iFrame "Hinit".
+        iIntros (δf ℓres) "HPred HfRes".
+        iSpecialize ("Hf" $! (δf, ℓres) with "HPred HfRes").
+        iApply ("Hf"). }
+      iIntros (?) "Hv !>".
+      ewp_pure_steps.
+      (* call the waker function *)
+      ewp_bind_rule; simpl.
+      iApply (ewp_mono with "[Hwaker]"); [by iApply "Hwaker"|].
+      iIntros (?) "_ !>".
+      ewp_pure_steps.
+      by iAssumption. }
+    iIntros (?) "(%ℓ' & -> & Hj) !>".
+    ewp_pure_steps.
+    iInv N as "(% & Hℓ & Hds)" "Hclose".
+    iApply (ewp_store with "Hℓ").
+    iIntros "!> Hℓ !>".
+    iDestruct "Hds" as "[(_ & Hγ')|(% & _ & Hγ' & _)]".
+    2: {
+      (* impossible *)
+      by iDestruct (domain_state_disjoint with "Hγ Hγ'") as "%HFalse".
+    }
+    iMod (domain_state_join γ with "[$]") as "Hγ".
+    iMod (domain_state_fulfill with "Hγ") as "#Hγ".
+    iMod ("Hclose" with "[Hj Hℓ Hγ]") as "_".
+    { iNext. rewrite /domain_inv. 
+      iExists _. iFrame "Hℓ". iRight.
+      iExists _. iSplit; first by done.
+      iFrame "Hγ". by iLeft. }
+    iModIntro. by iAssumption.
+  Qed.
 
-Lemma spawn_scheduler_spec (I Φ : val -> iProp Σ) (init f: val) :
-  promiseInv -∗ I init -∗ (∀ δℓ, EWP (f #()) <| Coop δℓ |> {{ v, □ Φ v }}) -∗
-    EWP (spawn_scheduler init f) {{ v, □ Φ v }}.
-Proof.
-  iIntros "HInv Hinit Hf". rewrite /spawn_scheduler.
-  ewp_pure_steps.
-  ewp_bind_rule. simpl.
-  iApply (ewp_mono with "[HInv Hinit Hf]").
-  iApply (spawn_spec N with "[HInv Hinit Hf]").
-  { ewp_pure_steps. 
-    iApply (ewp_run init f I Φ with "[HInv Hinit Hf]"). iFrame.
-    iIntros (δ ℓres) "HfRes".
-    iSpecialize ("Hf" $! (δ, ℓres)).
-    (* a.d. TODO remove the stupid box true *)
-    iApply (ewp_mono with "Hf"). iIntros (?) "HΦ !>". by iFrame. }
-  iIntros (v) "(% & -> & Hjoin) !>".
-  ewp_pure_steps.
-  iApply (join_spec with "Hjoin").
-Qed.
+  Lemma spawn_scheduler2_spec δf ℓres (I Φ : val -> iProp Σ) (init f: val) :
+    ⊢ promiseInv -∗ 
+      I init -∗ 
+      (∀ δℓ, isTlvPred δℓ.1.1.2 I -∗ fiberResources (fst δℓ) (snd δℓ) -∗ EWP (f #()) <| Coop δℓ |> {{ v, □ Φ v ∗ fiberResources (fst δℓ) (snd δℓ) }}) -∗
+      fiberResources δf ℓres -∗ 
+        EWP (spawn_scheduler2 init f) <| Coop (δf, ℓres) |> {{ v, □ Φ v ∗ fiberResources δf ℓres }}.
+  Proof.
+    iIntros "HInv Hinit Hf HfRes". rewrite /spawn_scheduler2.
+    ewp_pure_steps.
+    (* Allocate domain ref and its invariant. *)
+    (* a.d. TODO bind rule does not work for binding ref *)
+    iApply (ewp_bind' (AppRCtx _)); [by done|simpl].
+    iApply (ewp_alloc); iIntros "!> %ℓ Hℓ".
+    iMod (domain_state_create N Njoin _ Φ with "Hℓ") as (γ δ) "((Hδ & #Hdr) & Hγ)".
+    iModIntro. ewp_pure_steps.
+    (* Create the register function. *)
+    iApply (ewp_bind' (AppRCtx _)); [by done|simpl].
+    iApply (ewp_mono with "[Hdr HInv Hinit Hf Hγ]").
+    { iApply (ewp_os_prot_mono _ ⊥); first iApply iEff_le_bottom.
+      iApply (make_register_spec with "HInv Hinit Hf Hdr Hγ"). }
+    iIntros (reg) "Hreg !>".
+    ewp_pure_steps.
+    (* Perform suspend effect to get back domain_state_set γ *)
+    ewp_bind_rule; simpl.
+    iApply (ewp_mono with "[Hreg HfRes]").
+    { iApply ewp_suspend. iFrame. }
+    iIntros (?) "(HfRes & _ & Hγ) !>".
+    ewp_pure_steps.
+    (* Match the domain ref and contradict the second case. *)
+    ewp_bind_rule; simpl.
+    rewrite /is_domain_ref.
+    iApply (ewp_atomic ⊤ (⊤ ∖ ↑N)).
+    iMod (inv_acc with "Hdr") as "(Hd & Hclose)"; first by done.
+    iModIntro.
+    iDestruct "Hd" as "(% & Hℓ & [(_ & Hγ')|(%ℓ' & Heq & Hγ' & [Hj|Hδ'])])".
+    1: {
+      (* impossible *)
+      iApply (ewp_load with "Hℓ").
+      iIntros "!>".
+      by iDestruct (domain_state_disjoint with "Hγ' Hγ") as "%HFalse". 
+    }
+    2: {
+      (* impossible *)
+      iApply (ewp_load with "Hℓ").
+      iIntros "!>".
+      iCombine "Hδ Hδ'" as "H".
+      iPoseProof (own_valid with "H") as "%H".
+      destruct (exclusive_l _ _ H).
+    }
+    iApply (ewp_load with "Hℓ").
+    iIntros "!> Hℓ !>".
+    iDestruct "Heq" as "->".
+    iMod ("Hclose" with "[Hδ Hℓ Hγ']") as "_".
+    { 
+      iNext. rewrite /domain_inv.
+      iExists _. iFrame "Hℓ". iRight.
+      iExists _. iSplit; first done.
+      by iFrame.
+    }
+    iModIntro.
+    ewp_pure_steps.
+    iApply (ewp_mono with "[Hj]").
+    { iApply (ewp_os_prot_mono); [iApply iEff_le_bottom|].
+      iApply (join_spec with "Hj"). }
+    iIntros (?) "Hv !>".
+    iFrame.
+  Qed.
 
 End proof.
