theories/case_studies/eio/concurrent_queue.v
@@ -1,39 +1,63 @@
-From iris.base_logic.lib Require Import iprop.
+From iris.base_logic.lib Require Import iprop invariants.
 From program_logic Require Import reasoning_rules.
 
 Section concurrent_queue.
 Context `{!heapGS Σ}.
+Context (N : namespace).
 
+Parameter queue_change_state : val.
 Parameter queue_create : val.
 Parameter queue_push   : val.
 Parameter queue_pop    : val.
 
 Parameter is_queue :
-  val -d> (val -d> iPropO Σ) -d> iPropO Σ.
-  
+  valO -d> (valO -d> iPropO Σ) -d> iPropO Σ.
+Parameter is_queue_reader :
+  valO -d> (valO -d> iPropO Σ) -d> iPropO Σ.
+
+Parameter push_permission :
+  gnameO -d> iPropO Σ -d> iPropO Σ.
+Parameter fulfill_permission :
+  iPropO Σ -d> iPropO Σ.
+
 Parameter is_queue_ne_proof : ∀ (q: val) (n: nat),
   Proper ((dist n) ==> (dist n)) (is_queue q).
 
-Parameter is_queue_proper_proof : ∀ (q: val),
-  Proper ((≡) ==> (≡)) (is_queue q).
-
-Parameter is_queue_Persistent_proof : ∀ (q: val) (I: val -> iProp Σ),
+Parameter is_queue_Persistent_proof : ∀ (q : val) (I : val -> iProp Σ),
   Persistent (is_queue q I).
 
-Parameter queue_create_spec : ∀ (Ψ1 Ψ2: iEff Σ),
-  ⊢ EWP queue_create #() <| Ψ1 |> {| Ψ2 |} {{ q,
-      ∀ I, is_queue q I }}.
+Parameter is_queue_reader_ne_proof : ∀ (q: val) (n: nat),
+  Proper ((dist n) ==> (dist n)) (is_queue_reader q).
 
-Parameter queue_push_spec : ∀ (Ψ1 Ψ2: iEff Σ) (q: val) (I: val -> iProp Σ) v,
-  is_queue q I -∗
-    I v -∗
-      EWP queue_push q v <| Ψ1 |> {| Ψ2 |} {{ _, True }}.
+Parameter queue_register_push : ∀ (Q : iProp Σ) (q : val) (I: val -> iProp Σ),
+  ⊢ is_queue_reader q I -∗
+      EWP queue_change_state #() {{ _, 
+        is_queue q I ∗
+        fulfill_permission Q ∗
+        ∃ γ, push_permission γ Q }}.
 
-Parameter queue_pop_spec : ∀ (Ψ1 Ψ2: iEff Σ) (q: val) (I: val -> iProp Σ),
-  is_queue q I -∗
-    EWP queue_pop q <| Ψ1 |> {| Ψ2 |} {{ y,
-      ⌜ y = NONEV ⌝ ∨ 
-      ∃ (v: val), ⌜ y = SOMEV v ⌝ ∗ I v }}.
+Parameter queue_fulfill_Q : ∀ (Q : iProp Σ) (q : val) (I : val -> iProp Σ),
+  ⊢ is_queue q I -∗
+    fulfill_permission Q -∗
+    □ Q -∗
+      EWP queue_change_state #() {{ _, is_queue_reader q I }}.
+
+Parameter queue_create_spec :
+  ⊢ EWP queue_create #() {{ q, ∀ (I : val -> iProp Σ),
+      |={⊤}=> is_queue_reader q I }}.
+
+Parameter queue_push_spec : ∀ (γ : gname) (Q : iProp Σ) (I : val -> iProp Σ) (q : val) v,
+  ⊢ is_queue q I -∗ 
+    push_permission γ Q -∗
+    ▷ (Q -∗ I v) -∗
+      EWP queue_push q v {{ _, True }}.
+
+Parameter queue_pop_spec : ∀ (I: val -> iProp Σ) (q: val),
+  is_queue_reader q I -∗
+    EWP queue_pop q {{ ov, is_queue_reader q I ∗ (
+        ⌜ ov = NONEV ⌝ 
+      ∨ ∃ (v: val), ⌜ ov = SOMEV v ⌝ ∗ I v 
+    ) }}.
 
 Global Instance is_queue_ne q n:
   Proper ((dist n) ==> (dist n)) (is_queue q).
@@ -41,16 +65,16 @@ Proof.
   apply is_queue_ne_proof.
 Qed.
 
-Global Instance is_queue_proper q :
-  Proper ((≡) ==> (≡)) (is_queue q).
-Proof.
-  apply is_queue_proper_proof.
-Qed.
-
-Global Instance is_queue_Persistent q I:
+Global Instance is_queue_Persistent q I :
   Persistent (is_queue q I).
 Proof.
   apply is_queue_Persistent_proof.
+Qed.
+
+Global Instance is_queue_reader_ne q n:
+  Proper ((dist n) ==> (dist n)) (is_queue_reader q).
+Proof.
+  apply is_queue_reader_ne_proof.
 Qed.
 
 End concurrent_queue.
