theories/case_studies/eio/example.v
@@ -1,0 +1,367 @@
+From iris.proofmode Require Import base tactics classes.
+From iris.algebra Require Import excl_auth gset gmap agree csum frac excl.
+From iris.base_logic Require Import invariants.
+From iris.base_logic.lib Require Import iprop wsat saved_prop.
+From program_logic Require Import reasoning_rules.
+From case_studies Require Import list_lib .
+From case_studies.eio Require Import eio.
+From case_studies.mt Require Import spawn domain_manager.
+
+Section simple.
+  Context `{AsyncCompLib}.
+  
+  Existing Instance promise_inv_Persistent.
+
+  Definition simple_dispatch : val := (λ: <>, 
+    #1
+  )%V.
+  Definition simple_main : val := (λ: <>, 
+    let: "p" := fork_promise simple_dispatch in
+    let: "r" := await "p" in
+    "r"
+  )%V.
+
+  Lemma ewp_simple_dispatch δ ℓres : 
+    ⊢ EWP simple_dispatch #() <| coop (δ, ℓres) |> {{ v, ⌜ v = #1 ⌝ }}.
+  Proof.
+    iIntros.
+    rewrite /simple_dispatch.
+    ewp_pure_steps.
+    done.
+  Qed.
+    
+  Lemma ewp_simple_main δ ℓres : 
+    fiber_resources δ ℓres ∗ promise_inv
+    ⊢ EWP simple_main #() <| coop (δ, ℓres) |> {{ v, ⌜ v = #1 ⌝ }}.
+  Proof.
+    iIntros "(HfRes & #HpInv)".
+    rewrite /simple_main. ewp_pure_steps.
+    ewp_bind_rule; simpl.
+    iApply (ewp_mono _ _ with "[HfRes]"). 
+    { iApply fork_spec. iFrame. iSplit; first by done.
+      iIntros "HfRes". iApply (ewp_mono). iApply ewp_simple_dispatch.
+      iIntros (?) "-> !>".
+      Unshelve. 2: exact (λ v, ⌜ v = #1 ⌝%I).
+      simpl. iSplit; first done. done.
+    }
+    iIntros (p) "(Hp & HfRes) !>".
+    ewp_pure_steps.
+    ewp_bind_rule; simpl.
+    iApply (ewp_mono with "[HfRes Hp]").
+    { iApply await_spec. iFrame. by iAssumption. }
+    iIntros (?) "(-> & HfRes) !>".
+    ewp_pure_steps.
+    done.
+  Qed.
+End simple.
+
+Section complex.
+  (* main fiber spawns N schedulers in other threads and collects their results. *)
+
+  (* fiber that gets spawned in a new thread *)
+  Definition work : val := (λ: "seed" <>,
+    yield #();;
+    "seed"
+  )%V.
+
+  (* fiber that spawns the given "f" in a new thread. *)
+  Definition spawnwork : val := (λ: "f",
+    fork_promise (λ: <>, spawn_scheduler2 #() "f")
+  )%V.
+
+  Definition wait_for_data : val := (rec: "loop" "ctx" := 
+    match: Load "ctx" with
+      NONE => yield #();; "loop" "ctx"
+    | SOME "data" => "data"
+    end)%V.
+
+  (* fiber that forks "spawnwork" multiple times. *)
+  Definition dispatch : val := (λ: <>,
+    let: "ctx" := get_context #() in
+    let: "data" := wait_for_data "ctx" in
+    let: "p1" := spawnwork (work (Fst "data")) in 
+    let: "p2" := spawnwork (work (Snd "data")) in 
+    let: "r1" := await "p1" in
+    let: "r2" := await "p2" in
+    "r1" + "r2"
+  )%V.
+
+  Definition main_fiber : val := (λ: "i1" "i2" <>, 
+    let: "p" := fork_promise dispatch in
+    let: "ctx" := get_context #() in
+    "ctx" <- SOME ("i1", "i2");;
+    await "p"
+  )%V.
+
+  Definition main : val := (λ: <>,
+    let: "f" := main_fiber #17 #25 in
+    run NONEV "f"
+  )%V.
+Section complex.
+
+Class exampleG Σ := {
+  tlvContentG :> inG Σ (agreeR (prodO ZO ZO))
+}.
+
+Definition exampleΣ := #[
+  GFunctor (agreeR (prodO ZO ZO))
+].
+
+Instance subG_exampleΣ {Σ} : subG exampleΣ Σ → exampleG Σ.
+Proof. solve_inG. Qed.
+
+Section spec.
+  Context `{!exampleG Σ}.
+
+  Definition tlvContent γ (i1 i2 : Z) := own γ (to_agree (i1, i2)).
+  Definition tlvI γ (v : val) : iProp Σ := (
+    ⌜ v = NONEV ⌝ ∨ ∃ (i1 i2 : Z), ⌜ v = SOMEV (PairV #i1 #i2) ⌝ ∗ tlvContent γ i1 i2
+  )%I.
+
+  Lemma tlvContent_create i1 i2 :
+    ⊢ |==> ∃ γ, tlvContent γ i1 i2.
+  Proof. by iMod (own_alloc (to_agree (i1, i2))) as (γ) "Htlvc"; last iExists γ. Qed.
+
+  Lemma tlvContent_agree γ i1 i1' i2 i2' :
+    ⊢ tlvContent γ i1 i2 -∗ tlvContent γ i1' i2' -∗ ⌜ i1 = i1' ∧ i2 = i2' ⌝.
+  Proof.
+    iIntros "H H'". 
+    iCombine "H H'" as "H".
+    iPoseProof (own_valid with "H") as "%".
+    iPureIntro.
+    pose proof (to_agree_op_inv_L _ _ H) as H'.
+    by injection H'.
+  Qed.
+End spec.
+
+Section proof.
+  Context `{!heapGS Σ, !promiseGS Σ, !savedPredG Σ val, !spawnG Σ, !domainG Σ, !exampleG Σ}.
+  
+  Existing Instance promise_inv_Persistent.
+  Existing Instance tlv_agree_Persistent.
+  Existing Instance is_promise_Persistent.
+
+  Lemma ewp_work (n : Z) :
+    ⊢ EWP (work #n) {{f, ∀ δ ℓres, fiberResources δ ℓres -∗
+        EWP f #() <| Coop (δ, ℓres) |> {{v, □ ⌜ v = #n ⌝ ∗ fiberResources δ ℓres }}
+      }}.
+  Proof.
+    rewrite /work.
+    ewp_pure_steps.
+    iIntros (δ ℓres) "HfRes".
+    ewp_pure_steps.
+    ewp_bind_rule; simpl.
+    iApply (ewp_mono with "[HfRes]"); [iApply (ewp_yield with "HfRes")|].
+    iIntros (?) "HfRes !>".
+    ewp_pure_steps. 
+    by iFrame.
+  Qed.
+
+  Context (N Njoin : namespace).
+
+  Lemma ewp_spawnwork δ ℓres (f : val) Φ :
+    ⊢ promiseInv -∗ 
+      fiberResources δ ℓres -∗
+      (∀ δ' ℓres', fiberResources δ' ℓres' -∗ EWP f #() <| Coop (δ', ℓres') |> {{v, □ Φ v ∗ fiberResources δ' ℓres' }}) -∗ 
+        EWP (spawnwork f) <| Coop (δ, ℓres) |> {{v, 
+          ∃ (p: loc), ⌜ v = #p ⌝ ∗ isPromise p Φ ∗ fiberResources δ ℓres}}.
+  Proof.
+    iIntros "#HInv HfRes Hf".
+    rewrite /spawnwork.
+    ewp_pure_steps.
+    iApply (ewp_fork_promise).
+    iFrame "HfRes HInv".
+    iIntros "HfRes".
+    ewp_pure_steps.
+    iApply (spawn_scheduler2_spec N Njoin _ _ (λ _, True)%I Φ #() f with "HInv [] [Hf]").
+    - by done.
+    - iIntros "% _ HfRes".
+      destruct δℓ as [δ' ℓres'].
+      iSpecialize ("Hf" $! δ' ℓres' with "HfRes").
+      iApply (ewp_mono with "[Hf]"); [iApply "Hf"|].
+      iIntros (?) "HΦ !>".
+      by iFrame.
+    - by iFrame.
+  Qed.
+
+  Lemma ewp_wait_for_data γ δ ℓres ℓtlv :
+    ⊢ isTlvPred δ.1.2 (tlvI γ) -∗ 
+      tlvAgree δ.1.1 ℓtlv -∗
+      fiberResources δ ℓres -∗
+        EWP wait_for_data #ℓtlv <| Coop (δ, ℓres) |> {{v, fiberResources δ ℓres ∗ ∃ (i1 i2 : Z), ⌜ v = (PairV #i1 #i2) ⌝ ∗ tlvContent γ i1 i2 }}.
+  Proof.
+    iIntros "#HPred #HℓtlvAg HfRes".
+    rewrite /wait_for_data.
+    iLöb as "IH".
+    ewp_pure_steps.
+    destruct δ as [[δ11 δ12] δ2].
+    iDestruct "HfRes" as "((%ℓtlv' & #HℓtlvAg' & % & % & #HPred' & Hℓtlv & HI) & HRest)".
+    rewrite /tlvAgree /isTlvPred.
+    iDestruct (tlvAgree_agree with "HℓtlvAg HℓtlvAg'") as "->".
+    iDestruct (saved_pred_agree _ _ _ v with "HPred HPred'") as "Heq".
+    ewp_bind_rule; simpl.
+    iApply (ewp_load with "Hℓtlv").
+    iIntros "!> Hℓtlv !>".
+    iRewrite -"Heq" in "HI".
+    rewrite /tlvI.
+    iDestruct "HI" as "[->|(%&%&->&#Hi)]".
+    - ewp_pure_steps.
+      ewp_bind_rule; simpl.
+      iApply (ewp_mono with "[Hℓtlv HRest]").
+      { iApply (ewp_yield with "[Hℓtlv HRest]").
+        iFrame "HRest". iExists ℓtlv'.
+        rewrite /isFiberContext.
+        simpl.
+        repeat iSplit; try done.
+        iExists (InjLV #()), (tlvI γ). 
+        repeat iSplit; try done.
+        by iLeft. }
+      iIntros (?) "HfRes !>".
+      do 3 ewp_value_or_step.
+      iApply ("IH" with "HfRes").
+    - ewp_pure_steps.
+      iSplitL. 
+      { iFrame "HRest". iExists ℓtlv'.
+        rewrite /isFiberContext.
+        simpl.
+        repeat iSplit; try done.
+        iExists (InjRV (PairV #i1 #i2)), (tlvI γ). 
+        repeat iSplit; try done.
+        rewrite /tlvI.
+        iRight. iExists _, _.
+        repeat iSplit; try done. }
+      iExists _, _. by iSplit.
+  Qed.
+
+  Lemma ewp_dispach γ δ ℓres i1 i2 : 
+    ⊢ promiseInv -∗
+      isTlvPred δ.1.2 (tlvI γ) -∗
+      tlvContent γ i1 i2 -∗ 
+      fiberResources δ ℓres -∗
+        EWP dispatch #() <| Coop (δ, ℓres) |> {{v, ⌜ v = #(i1 + i2) ⌝ ∗ fiberResources δ ℓres }}.
+  Proof.
+    iIntros "#HInv #HPred #Htlvc HfRes".
+    rewrite /dispatch.
+    ewp_pure_steps.
+    (* get context *)
+    ewp_bind_rule; simpl.
+    iApply (ewp_mono); [iApply (ewp_get_context)|].
+    iIntros (?) "(%ℓtlv & -> & #HℓtlvAg) !>".
+    ewp_pure_steps.
+    (* wait until tlv is filled *)
+    ewp_bind_rule; simpl.
+    iApply (ewp_mono with "[HfRes]"); [iApply (ewp_wait_for_data with "HPred HℓtlvAg HfRes")|].
+    iIntros (?) "(HfRes&%i1'&%i2'&->&#Htlvc') !>".
+    iDestruct (tlvContent_agree with "Htlvc Htlvc'") as "[<- <-]".
+    ewp_pure_steps.
+    (* p1 *)
+    ewp_bind_rule; simpl.
+    iApply (ewp_mono).
+    { iApply ewp_os_prot_mono; [iApply iEff_le_bottom|iApply (ewp_work i1)]. }
+    iIntros (f1) "Hf1 !>".
+    ewp_bind_rule; simpl.
+    iApply (ewp_mono with "[Hf1 HfRes]"); [iApply (ewp_spawnwork with "HInv HfRes Hf1")|].
+    iIntros (?) "(%p1 & -> & Hp1 & HfRes) !>".
+    ewp_pure_steps.
+    (* p2 *)
+    ewp_bind_rule; simpl.
+    iApply (ewp_mono).
+    { iApply ewp_os_prot_mono; [iApply iEff_le_bottom|iApply (ewp_work i2)]. }
+    iIntros (f2) "Hf2 !>".
+    ewp_bind_rule; simpl.
+    iApply (ewp_mono with "[Hf2 HfRes]"); [iApply (ewp_spawnwork with "HInv HfRes Hf2")|].
+    iIntros (?) "(%p2 & -> & Hp2 & HfRes) !>".
+    ewp_pure_steps.
+    (* r1 *)
+    ewp_bind_rule; simpl.
+    iApply (ewp_mono with "[Hp1 HfRes]"); [iApply (ewp_await with "[$]")|].
+    iIntros (r1) "(-> & HfRes) !>". 
+    ewp_pure_steps.
+    (* r2 *)
+    ewp_bind_rule; simpl.
+    iApply (ewp_mono with "[Hp2 HfRes]"); [iApply (ewp_await with "[$]")|].
+    iIntros (r2) "(-> & HfRes) !>". 
+    ewp_pure_steps.
+    (* calculate *)
+    by reflexivity.
+    by iFrame.
+  Qed.
+
+  Lemma ewp_main_fiber γ i1 i2 : 
+    ⊢ promiseInv -∗
+      tlvContent γ i1 i2 -∗ 
+        EWP main_fiber #i1 #i2 {{f, 
+          ∀ δ ℓres, isTlvPred δ.1.2 (tlvI γ) -∗ fiberResources δ ℓres -∗
+            EWP f #() <| Coop (δ, ℓres) |> {{v, □ ⌜ v = #(i1 + i2) ⌝ ∗ fiberResources δ ℓres }}
+        }}.
+  Proof.
+    iIntros "#HInv #Htlvc".
+    rewrite /main_fiber.
+    ewp_pure_steps.
+    iIntros (? ?) "#HPred HfRes".
+    ewp_pure_steps.
+    ewp_bind_rule; simpl.
+    iApply (ewp_mono with "[HfRes]").
+    { iApply (ewp_fork_promise _ _ (λ v, ⌜ v = #(i1 + i2) ⌝)%I).
+      iFrame "HfRes HInv".
+      iIntros "HfRes".
+      iApply (ewp_mono with "[HfRes]").
+      iApply (ewp_dispach with "HInv HPred Htlvc HfRes").
+      iIntros (?) "(-> & HfRes) !>".
+      by iFrame. }
+    iIntros (?) "(% & -> & #HisPr & HfRes) !>".
+    ewp_pure_steps.
+    (* get context *)
+    ewp_bind_rule; simpl.
+    iApply (ewp_mono); [iApply (ewp_get_context)|].
+    iIntros (?) "(%ℓtlv & -> & #HℓtlvAg) !>".
+    iDestruct "HfRes" as "((%ℓtlv' & #HℓtlvAg' & % & % & #HPred' & Hℓtlv & _) & HRest)".
+    iDestruct (tlvAgree_agree with "HℓtlvAg HℓtlvAg'") as "->".
+    (* iDestruct (saved_pred_agree _ _ _ v with "HPred HPred'") as "Heq". *)
+    ewp_pure_steps.
+    ewp_bind_rule; simpl.
+    iApply (ewp_store with "Hℓtlv").
+    iIntros "!> Hℓtlv !>".
+    ewp_pure_steps.
+    (* await the result *)
+    iApply (ewp_mono with "[Hℓtlv HRest]").
+    { iApply (ewp_await with "[Hℓtlv HRest]").
+      iFrame "HInv HisPr HRest".
+      iExists ℓtlv'. 
+      iFrame "HℓtlvAg".
+      iExists _, _. iFrame "HPred Hℓtlv".
+      iRight. iExists _, _. by repeat iSplit. }
+    by iIntros (?) "(-> & $)".
+  Qed.
+End proof.
+
+Section closed.
+  Context `{!heapGS Σ, !promiseGpreS Σ, !savedPredG Σ val, !spawnG Σ, !domainG Σ, !exampleG Σ}.
+  Context (N Njoin : namespace).
+
+  Lemma ewp_main :
+    ⊢ EWP main #() {{v, ⌜ v = #42 ⌝ }}.
+  Proof.
+    rewrite /main.
+    ewp_pure_steps.
+    rewrite -fupd_ewp.
+    iMod (promiseInv_init) as (?) "#HInv".
+    iMod (tlvContent_create 17 25) as (γ) "#Htlvc".
+    iModIntro.
+    iApply (ewp_bind' (AppRCtx _)); [by done|simpl].
+    iApply (ewp_mono); [iApply (ewp_main_fiber N Njoin with "HInv Htlvc")|].
+    iIntros (f) "Hf !>".
+    ewp_pure_steps.
+    iApply (ewp_mono with "[Hf]").
+    iApply (ewp_run _ _ (tlvI γ) with "[Hf]").
+    iFrame "Hf".
+    by iLeft.
+    iIntros (?) "-> !>".
+    iPureIntro.
+    by compute.
+  Qed.
+End closed.
+
+
+  
+
